src/Points.v
@@ -1,4 +1,3 @@
-
 Require Export IndexedCodes.
 
 (** * Points as quotients of indexed codes.
@@ -24,37 +23,52 @@ Proof.
   auto.
 Qed.
 
-Notation "[ x ]" := (denote (codes_code x)) : point_scope.
-
-Definition point_le {Var : Set} (p p' : Point Var) :=
-  codes_le (access p) (access p').
-Definition point_eq {Var : Set} (p p' : Point Var) :=
-  codes_eq (access p) (access p').
-
-Notation "x [= y" := (point_le x y) : point_scope.
-Notation "x [=] y" := (point_eq x y) : point_scope.
+Notation "[ x ]" := (denote (codes_code x)%code) : point_scope.
 
 Open Scope point_scope.
 Delimit Scope point_scope with point.
 Bind Scope point_scope with Point.
 
+Definition definable {Var : Set} (p : Point Var) := {x : code & p = [x]}.
+
+Definition point_le {Var : Set} (p p' : Point Var) :=
+  codes_le (access p) (access p').
+
+Notation "x [= y" := (point_le x y)%point : point_scope.
+
 Definition point_ap {Var : Set} (p p' : Point Var) :=
   denote (codes_ap (access p) (access p')).
-Infix "*" := point_ap : point_scope.
 
-Notation "'TOP'" := [code_top] : point_scope.
-Notation "'BOT'" := [code_bot] : point_scope.
-Notation "'J'" := [code_j] : point_scope.
-Notation "'I'" := [code_i] : point_scope.
-Notation "'K'" := [code_k] : point_scope.
-Notation "'B'" := [code_b] : point_scope.
-Notation "'C'" := [code_c] : point_scope.
-Notation "'S'" := [code_s] : point_scope.
-Notation "p * p'" := (point_ap p p')%point : point_scope.
+Definition point_sub {Var Var' : Set} (f : Var -> Point Var') (x : Point Var)
+  : Point Var' :=
+  denote (codes_sub (fun v => access (f v)) (access x)).
+
+Definition point_sup {Var : Set} {i : Type} (e : i -> Point Var) : Point Var.
+Proof.
+  apply denote; apply direct; unfold Precodes.
+Admitted.
+
+Notation "'TOP'" := [TOP] : point_scope.
+Notation "'BOT'" := [BOT] : point_scope.
+Notation "'J'" := [J] : point_scope.
+Notation "'R'" := [R] : point_scope.
+Notation "'I'" := [I] : point_scope.
+Notation "'K'" := [K] : point_scope.
+Notation "'B'" := [B] : point_scope.
+Notation "'C'" := [C] : point_scope.
+Notation "'S'" := [S] : point_scope.
+Notation "'Y'" := [Y] : point_scope.
+Notation "'V'" := [V] : point_scope.
+Notation "x * y" := (point_ap x y)%point : point_scope.
+Notation "x 'o' y" := (B * x * y)%point : point_scope.
 Notation "x || y" := (J * x * y)%point : point_scope.
+Notation "x (+) y" := (R * x * y)%point : point_scope.
+Notation "x @ f" := (point_sub f x)%point : point_scope.
 
-Definition sup {Var : Set} {i : Type} (e : i -> Code Var) : Point Var :=
-  denote (codes_sup e).
+Definition point_nle {Var : Set} (x y : Point Var) : Prop :=
+  exists (Var' : Set) (c : Point Var') (f : Var -> Point Var'),
+    c * (x @ f) = TOP /\ c * (y @ f) = BOT.
+Notation "x [!= y" := (point_nle x y)%point : point_scope.
 
 Lemma point_ap_respect (Var : Set) (x y : Code Var) : [x] * [y] = [x * y]%code.
 Proof.
@@ -62,9 +76,323 @@ Proof.
   (* TODO *)
 Admitted.
 
+Lemma point_sub_respect (Var Var' : Set) (f : Var -> Code Var') (x : Code Var)
+  : [x] @ (fun v => [f v]%code) = [x @ f]%code.
+Proof.
+  unfold point_sub; unfold codes_sub.
+  (* TODO *)
+Admitted.
+
+(** Local properties of points *)
+
+Section point_beta.
+  Variable Var : Set.
+  Variable w x y z : Point Var.
+
+  Lemma point_i_beta : I * x = x.
+  Admitted.
+
+  Lemma point_k_beta : K * x * y = x.
+  Admitted.
+
+  Lemma point_b_beta : B * x * y * z = x * (y * z).
+  Admitted.
+
+  Lemma point_c_beta : C * x * y * z = x * z * y.
+  Admitted.
+
+  Lemma point_s_beta : S * x * y * z = x * z * (y * z).
+  Admitted.
+
+  Lemma point_j_beta : (x || y) * z = x * z || y * z.
+  Admitted.
+
+  Lemma point_r_beta : (x (+) y) * z = x * z (+) y * z.
+  Admitted.
+
+  Lemma point_r_idem : x (+) x = x.
+  Admitted.
+
+  Lemma point_r_sym : x (+) y = y (+) x.
+  Admitted.
+
+  Lemma point_r_sym_sym : (w(+)x) (+) (y(+)z) = (y(+)x) (+) (w(+)z).
+  Admitted.
+
+  Variable index : Type.
+  Variable e : index -> Point Var.
+
+  Lemma point_sup_beta : point_sup e * y = point_sup (e i * y for i : index).
+  Admitted.
+End point_beta.
+
+Hint Rewrite
+  point_i_beta point_k_beta point_b_beta point_c_beta
+  point_s_beta point_j_beta point_r_beta point_r_idem point_sup_beta
+  : beta.
+
+Tactic Notation "beta_reduce" := autorewrite with beta.
+Tactic Notation "beta_reduce" "in" hyp(H) := autorewrite with beta in H.
+
+(** To avoid nontermination in [beta_reduce],
+    we provide a mechanism to "freeze" terms during reduction. *)
+Tactic Notation "freeze" reference(c) "in" tactic(tac) :=
+  let v := fresh "v" in
+  let H := fresh "Hv" in
+  assert (exists v, c=v) as H;
+  [ exists c; reflexivity
+  | destruct H as [v H]; rewrite H; tac; destruct H].
+
+Section point_algebra.
+  Variable Var : Set.
+  Variable x x' y y' z : Point Var.
+
+  Lemma point_le_top : x [= TOP.
+  Admitted.
+
+  Lemma point_le_bot : BOT [= x.
+  Admitted.
+
+  Lemma point_j_left : x [= x || y.
+  Admitted.
+
+  Lemma point_j_right : y [= x || y.
+  Admitted.
+
+  Lemma point_j_lub : x [= z -> y [= z -> x || y [= z.
+  Admitted.
+
+  Lemma point_r_subconvex : x [= z -> y [= z -> x(+)y [= z.
+  Admitted.
+
+  Lemma point_r_supconvex : z [= x -> z [= x -> z [= x(+)y.
+  Admitted.
+
+  Lemma point_le_refl : x [= x.
+  Admitted.
+
+  Lemma point_le_antisym : x [= y -> y [= x -> x = y.
+  Admitted.
+
+  Lemma point_le_trans : x [= y -> y [= z -> x [= z.
+  Admitted.
+
+  Lemma point_le_ap_left : x [= x' -> x * y [= x' * y.
+  Admitted.
+
+  Lemma point_le_ap_right : y [= y' -> x * y [= x * y'.
+  Admitted.
+
+  Lemma point_le_ap : x [= x' -> y [= y' -> x * y [= x' * y'.
+  Admitted.
+End point_algebra.
+
+Hint Resolve point_le_top.
+Hint Resolve point_le_bot.
+Hint Resolve point_j_left.
+Hint Resolve point_j_right.
+Hint Resolve point_j_lub.
+Hint Resolve point_le_refl.
+Hint Resolve point_le_antisym.
+Hint Resolve point_le_ap_left.
+Hint Resolve point_le_ap_right.
+Hint Resolve point_le_ap.
+
+Ltac monotonicity := repeat (
+  apply point_le_ap_left ||
+  apply point_le_ap_right ||
+  apply point_le_ap).
+
+(** Properties of [sup] *)
+
+Section point_join.
+  Variable Var : Set.
+  Variable x y z : Point Var.
+
+  Lemma point_join_sym : x || y = y || x.
+  Proof.
+    auto.
+  Qed.
+
+  Lemma point_le_eq_join : x [= y <-> x || y = y.
+  Proof.
+    split; intro H.
+    apply point_le_antisym; auto.
+    rewrite <- H; auto.
+  Qed.
+End point_join.
+
+Definition is_upper_bound {Var : Set} {s : Type}
+  (e : s -> Point Var) (x : Point Var) : Prop :=
+  forall i, e i [= x.
+
+Definition is_lub {Var : Set} {s : Type}
+  (e : s -> Point Var) (x : Point Var) : Prop :=
+  is_upper_bound e x /\ forall y, is_upper_bound e y -> x [= y.
+
+Section point_sup_lub.
+  Variable Var : Set.
+  Variable index : Type.
+  Variable e : index -> Point Var.
+
+  Lemma point_sup_lub : is_lub e (point_sup e).
+  Admitted.
+
+  Lemma point_sup_ub : forall i, e i [= point_sup e.
+  Proof.
+    apply point_sup_lub.
+  Qed.
+
+  Lemma point_sup_ub_eq : forall i x, x = e i -> x [= point_sup e.
+  Proof.
+    intros i x Heq; rewrite Heq; apply point_sup_lub.
+  Qed.
+End point_sup_lub.
+
+Section point_sup_empty.
+  Variable Var : Set.
+
+  Lemma point_sup_empty (e : Empty_set -> Point Var) : point_sup e = BOT.
+  Proof.
+    apply point_le_antisym.
+      apply point_sup_lub; unfold is_upper_bound; intro i; elim i.
+    auto.
+  Qed.
+
+  Lemma point_sup_single (x : Point Var) (s : Type) :
+    s -> point_sup (x for _ : s) = x.
+  Proof.
+    intros y.
+    apply point_le_antisym;
+    apply point_sup_lub with (e := fun _ : s => x);
+    unfold is_upper_bound;
+    auto.
+  Qed.
+End point_sup_empty.
+
+(** Global properties of [Points] *)
+
 Theorem consistency (Var : Set) : [@code_top Var] <> [@code_bot Var].
 Proof.
   (* TODO apply access_denote. *)
 Admitted.
 
-Definition definable {Var : Set} (p : Point Var) := {x : code & p = [x]}.
+Theorem completeness (Var : Set) (s : Type) (e : s -> Point Var) :
+  exists x, is_lub e x.
+Proof.
+  exists (point_sup e); apply point_sup_lub.
+Qed.
+
+Theorem extensionality (Var : Set) (f g : Point Var) :
+  (forall x, f * x = g * x) -> f = g.
+Proof.
+  (* TODO *)
+Admitted.
+
+Corollary point_le_extensionality (Var : Set) (f g : Point Var) :
+  (forall x, f * x [= g * x) -> f [= g.
+Proof.
+  intros H.
+  apply point_le_eq_join.
+  apply extensionality; intro x.
+  rewrite point_j_beta; auto.
+Qed.
+
+(** ** Example reasoning using beta-eta conversion *)
+
+Tactic Notation "eta_expand" :=
+  let x := fresh in
+  match goal with
+  | [|- _ = _] => apply extensionality; intro x
+  | [|- _ [= _] => apply point_le_extensionality; intro x
+  end.
+
+Tactic Notation "eta_expand" "as" ident(x) :=
+  match goal with
+  | [|- _ = _] => apply extensionality; intro x
+  | [|- _ [= _] => apply point_le_extensionality; intro x
+  end.
+
+Tactic Notation "eta_expand" "in" hyp(H) :=
+  eapply point_le_ap_left in H; beta_reduce in H.
+
+Ltac beta_eta :=
+  simpl; (
+  beta_reduce; auto
+  || eta_expand; beta_reduce; auto
+  || eta_expand; eta_expand; beta_reduce; auto
+  || eta_expand; eta_expand; eta_expand; beta_reduce; auto).
+
+Section point_b_assoc.
+  Variable Var : Set.
+  Variable x y z : Point Var.
+
+  Lemma point_b_assoc : (x o y) o z = x o (y o z).
+  Proof.
+    beta_eta.
+  Qed.
+
+  Lemma point_beta_top : TOP * x = TOP.
+  Proof.
+    apply point_le_antisym.
+    apply point_le_top.
+    apply point_le_trans with (K * TOP * x).
+    beta_eta.
+    apply point_le_ap_left; auto.
+  Qed.
+
+  Lemma point_beta_bot : BOT * x = BOT.
+  Proof.
+    apply point_le_antisym.
+    apply point_le_trans with (K*BOT*x).
+    apply point_le_ap_left; auto.
+    beta_eta.
+    apply point_le_bot.
+  Qed.
+
+  Lemma point_beta_join_top_left : TOP || x = TOP.
+  Proof.
+    rewrite point_join_sym; apply point_le_eq_join; auto.
+  Qed.
+
+  Lemma point_beta_join_top_right : x || TOP = TOP.
+  Proof.
+    rewrite point_join_sym; apply point_beta_join_top_left.
+  Qed.
+
+  Lemma point_beta_join_bot_left : BOT || x = x.
+  Proof.
+    apply point_le_eq_join; auto.
+  Qed.
+
+  Lemma point_beta_join_bot_right : x || BOT = x.
+  Proof.
+    rewrite point_join_sym; apply point_beta_join_bot_left.
+  Qed.
+End point_b_assoc.
+
+Hint Rewrite
+  point_beta_top point_beta_bot
+  point_beta_join_top_left point_beta_join_top_right
+  point_beta_join_bot_left point_beta_join_bot_right
+  : beta.
+
+Lemma point_j_k_ki (Var : Set) : (J : Point Var) = K || K*I.
+Proof.
+  beta_eta.
+Qed.
+
+Section point_sup_pair.
+  Variable Var : Set.
+  Let bool_to_point (b : bool) : Point Var := if b then K else K * I.
+  Lemma point_sup_pair : J = point_sup bool_to_point.
+  Proof.
+    rewrite point_j_k_ki.
+    apply point_le_antisym.
+      apply point_j_lub.
+        apply point_sup_ub with (e := bool_to_point) (i := true).
+      apply point_sup_ub with (e := bool_to_point) (i := false).
+    apply point_sup_lub; unfold is_upper_bound.
+    intro b; case b; auto.
+  Qed.
+End point_sup_pair.
